Introduced hide and bang operator

examples/DenoteCCS.v
@@ -3,22 +3,28 @@ From ITree Require Import
      ITreeDefinition
      Interp.Traces
      Eq
-     .
+.
+
+From ExtLib Require Import
+     Structures.Functor
+     Structures.Monad.
 
 From Coq Require Import
-     Lists.List
      Arith.EqNat
      Arith.PeanoNat
-     Program.Equality
-     List
-     Setoid
+     Lists.List
      Morphisms
+     Program.Equality
+     Setoid
+     Strings.String
      RelationClasses
-     Relations.Relation_Operators.
+     Relations.Relation_Operators
+     ZArith.Int.
 
 From Paco Require Import paco.
 
 Require Import ITree.Eq.EqAxiom.
+Require Import Fin.
 
 (** * Modeling Concurrency with ITrees (CCS)
 
@@ -48,15 +54,12 @@ Set Primitive Projections.
   (** CCS Operators:
 
       P := ∅          Empty Process
-         | A = P1     Process Identifier *** (TODO)
          | a.P1       Action
          | P1 + P2    Choice (Sum type)
          | P1 ∥ P2    Parallel Composition
-         | P1 ∖ a     Restriction *** (TODO)
+         | P1 ∖ a     Restriction
 
       * Empty Process
-      * Process Identifier: Identifier A refers to process P1. Allows
-                            recursive definitions.
       * Action: Process P1 performs an action a. This could be a send or
                 receive, depending on the polarity of the action a.
       * Choice : either P1 or P2 will be processed.
@@ -68,483 +71,568 @@ Set Primitive Projections.
 (** *Denotation of CCS with ITrees *)
 Section ccs.
 
-(* We need a decidable equality on labels for the Restriction and Parallel
-   Composition operator. *)
+  (* Locally Nameless representation of variables. *)
+  Variant idx : Type :=
+  | I_string (s : string) : idx
+  | I_nat (n : nat) : idx
+  .
 
-Variable A : Type.
-Variable A_dec_eq : forall x y: A, {x = y} + {x <> y}.
+  Definition eq_idx : idx -> idx -> bool :=
+    fun i1 i2 =>
+      match i1 with
+      | I_string s => match i2 with
+                    | I_string s => true
+                    | _ => false
+                    end
+      | I_nat n => match i2 with
+                  | I_nat n => true
+                  | _ => false
+                  end
+      end
+  .
 
-Definition A_beq (a1 a2 : A): bool := true. (* TODO *)
+  (* Labels for defining parity of actions. *)
+  Variant Label : idx -> Type :=
+  | In (l : idx) : Label l
+  | Out (l : idx): Label l
+  .
 
-Variant Label : Type :=
-| In (l : A) : Label
-| Out (l : A) : Label.
+  (* We need a decidable equality on labels for the Restriction and Parallel
+  Composition operator. *)
+  Theorem label_dec_eq :
+    forall (l : idx) (x y : Label l), {x = y} + {x <> y}.
+  Proof.
+    intros.
+    destruct x, y;
+      repeat (
+    try (left; reflexivity);
+    try (right; intro; inversion H)).
+  Qed.
 
-Theorem label_dec_eq :
-  forall x y : Label, {x = y} + {x <> y}.
-Proof.
-  decide equality.
-Qed.
-
-(* Denotation of CCS Operators as ITree events. *)
-Variant ccsE : Type -> Type :=
-| Or (n : nat): ccsE nat (* Note: choices are zero-indexed. *)
-| Act : Label -> ccsE unit
-| Sync : A -> ccsE unit
-| Fail : ccsE void.
+  (* Denotation of CCS Operators as ITree events. *)
+  Variant ccsE : Type -> Type :=
+  | Or (n : nat) : ccsE nat
+     (* Note: choices are zero-indexed. *)
+  | Act (l : idx) : Label l -> ccsE unit
+  | Sync : idx -> ccsE unit
+  | Fail : ccsE void
+  .
 
 Definition ccs := itree ccsE unit.
 
+End ccs.
+
+(* begin hide *)
+Bind Scope ccs_scope with ccs.
+Delimit Scope ccs_scope with ccs.
+Local Open Scope ccs_scope.
+
+Arguments In {_}.
+Arguments Out {_}.
+(* end hide *)
+
 Notation ccs' := (itree' ccsE unit).
 
-(** Denotation of basic operations in CCS.
-    For now, we reason about finitary ITrees. *)
+Infix "≡?" := (eq_idx) (at level 70) : ccs_scope.
 
-(* The empty process. *)
-Definition zero : ccs := Ret tt. (* Or 0 as zero? *)
+Section ccs_combinators.
 
-Definition fail : ccs := Vis Fail (fun x : void => match x with end).
+  (** *Denotation of CCS Combinators *)
 
-(* Action operators, where l denotes the label. *)
-Definition send (l : A) (k : ccs) : ccs := Vis (Act (In l)) (fun _ => k).
+  (* The empty process. *)
+  Definition zero : ccs := Ret tt. (* Or 0 as zero? *)
 
-Definition recv (l : A) (k : ccs) : ccs := Vis (Act (Out l)) (fun _ => k).
+  Definition fail : ccs := Vis Fail (fun x : void => match x with end).
 
-(* Choose operator, where n is the number of choices. *)
-Definition pick (n: nat) (k : nat -> ccs) : ccs := Vis (Or n) k.
+  (* Action operators, where l denotes the label. *)
+  Definition send (l : idx) (k : ccs) : ccs := Vis (Act (@In l)) (fun _ => k).
 
-(* Parallel composition operator (#).
+  Definition recv (l : idx) (k : ccs) : ccs := Vis (Act (@Out l)) (fun _ => k).
 
-   (#) Follows denotation of CCS parallel composition operator from
-       Section 5 Rule IV. (p. 269) of:
-       M. Henessy & G. Plotkin, A Term Model for CCS, 1980. *)
-(* TODO: State invariant on atomic processes? *)
-CoFixpoint par (p1 p2 : ccs) : ccs :=
-  let par_left (p1 p2 : ccs) : ccs :=
-    match p1, p2 with
-    | (Vis (Act x) k), _ => Vis (Act x) (fun _ => par (k tt) p2)
-    | Vis (Sync a) t1, _ => Vis (Sync a) (fun _ => par (t1 tt) p2)
-    | Ret _, _ => Tau p2
-    | _, _ => fail
-    end
-  in let par_right (p1 p2 : ccs) : ccs :=
-    match p1, p2 with
-    | _, (Vis (Act x) k) => Vis (Act x) (fun _ => par p1 (k tt))
-    | _, Vis (Sync a) t1 => Vis (Sync a) (fun _ => par p1 (t1 tt))
-    | _, Ret _ => Tau p1
-    | _, _ => fail
-    end
-  in let par_comm (p1 p2 : ccs) : ccs :=
-    match p1, p2 with
-    | (Vis (Act (In l1)) k1), (Vis (Act (Out l2)) k2) =>
-      if A_beq l1 l2
-      then Vis (Sync l1) (fun _ => par (k1 tt) (k2 tt))
-      else fail
-    | (Vis (Act (Out l1)) k1), (Vis (Act (In l2)) k2) =>
-      if A_beq l1 l2
-      then Vis (Sync l1) (fun _ => par (k1 tt) (k2 tt))
-      else fail
-    | _, _ => fail
-    end
-  in
-  match (observe p1), (observe p2) with
-  | (VisF (Or n1) k1), (VisF (Or n2) k2) =>
+  (* Hide operator. *)
+  Definition hide' (l : idx) {E : Type -> Type}: ccsE ~> ccsE :=
+    fun _ e =>
+      match e with
+      | Act (@In n) => if n ≡? l then
+                        Act (@In (I_nat 0))
+                      else
+                        match n with
+                        | I_string _ => Act (@In n)
+                        | I_nat i => Act (@In (I_nat (i + 1)))
+                        end
+      | Act (@Out n) => if n ≡? l then
+                         Act (@In (I_nat 0))
+                       else
+                         match n with
+                         | I_string _ => Act (@Out n)
+                         | I_nat i => Act (@Out (I_nat (i + 1)))
+                         end
+      | x => x
+      end
+  .
+
+  Definition hide (l : idx) (t : ccs) : ccs :=
+    translate (@hide' l ccsE) t.
+
+  (* Choose operator, where n is the number of choices. *)
+  Definition pick (n : nat) (k : nat -> ccs) : ccs := Vis (Or n) k.
+
+
+  (* Parallel composition operator (#).
+
+    (#) Follows denotation of CCS parallel composition operator from
+        Section 5 Rule IV. (p. 269) of:
+        M. Henessy & G. Plotkin, A Term Model for CCS, 1980. *)
+  CoFixpoint par (p1 p2 : ccs) : ccs :=
+    let par_left (p1 p2 : ccs) : ccs :=
+      match p1, p2 with
+      | (Vis (Act x) k), _ => Vis (Act x) (fun _ => par (k tt) p2)
+      | Vis (Sync a) t1, _ => Vis (Sync a) (fun _ => par (t1 tt) p2)
+      | Ret _, _ => Tau p2
+      | _, _ => fail
+      end
+    in let par_right (p1 p2 : ccs) : ccs :=
+      match p1, p2 with
+      | _, (Vis (Act x) k) => Vis (Act x) (fun _ => par p1 (k tt))
+      | _, Vis (Sync a) t1 => Vis (Sync a) (fun _ => par p1 (t1 tt))
+      | _, Ret _ => Tau p1
+      | _, _ => fail
+      end
+    in let par_comm (p1 p2 : ccs) : ccs :=
+      match p1, p2 with
+      | (Vis (Act (@In l1)) k1), (Vis (Act (@Out l2)) k2) =>
+        if l1 ≡? l2
+        then Vis (Sync l1) (fun _ => par (k1 tt) (k2 tt))
+        else fail
+      | (Vis (Act (@Out l1)) k1), (Vis (Act (@In l2)) k2) =>
+        if l1 ≡? l2
+        then Vis (Sync l1) (fun _ => par (k1 tt) (k2 tt))
+        else fail
+      | _, _ => fail
+      end
+    in
+    match (observe p1), (observe p2) with
+    | (VisF (Or n1) k1), (VisF (Or n2) k2) =>
       Vis (Or (n1 + n2 + (n1 * n2))) (fun n0 : nat =>
-                    if beq_nat n0 n1
-                    then par_left (k1 n0) p2
-                    else if beq_nat n0 (n2 + n2)
-                         then par_right p1 (k2 (n0 - n1))
-                         else par_comm (k1 ((n0 - n1 - n2) mod n2)) (k2 ((n0 - n1 - n2) / n1)))
-  | _, _ => fail
-  end
+        if beq_nat n0 n1
+        then par_left (k1 n0) p2
+        else if beq_nat n0 (n2 + n2)
+          then par_right p1 (k2 (n0 - n1))
+          else par_comm (k1 ((n0 - n1 - n2) mod n2)) (k2 ((n0 - n1 - n2) / n1)))
+    | _, _ => fail
+    end
+  .
+
+  (** *Shape Invariant
+
+    The tree should alternate in depth starting with a (Vis (Or _) _)
+    node, then a non-(Vis (Or _) _) node, and keep alternating until
+    it finds a leaf.
+
+    The equational properties of CCS structural congruences state that
+    any level of the tree can be defined as a sum. This shape invariant
+    is necessary for our parallel composition operator, and we define this
+    shape as the canonical shape for our denotation of CCS with ITrees.
+  *)
+
+  (* Functorial definition of shape invariant.
+    The definition takes two parameters :
+    - [b] is a boolean flag indicating whether or not it is currently
+      at an [Or] event level of the tree.
+    - [inv] is the currently built coinductive relation.
+  *)
+  Inductive shape_invF (inv : bool -> ccs -> Prop) : bool -> ccs' -> Prop :=
+  | ShapeRet :
+      shape_invF inv false (RetF tt)
+  | ShapeOr k
+            (n1 n2 : nat)
+            (REL : forall n1, inv false (k n1)):
+      shape_invF inv true (VisF (Or n2) k)
+  | ShapeActIn a k
+              (REL : inv true (k tt)):
+      shape_invF inv false (VisF (Act (@In a)) k)
+  | ShapeActOut a k
+                (REL : inv true (k tt)):
+      shape_invF inv false (VisF (Act (@Out a)) k)
+  | ShapeSync a k
+              (REL : inv true (k tt)):
+      shape_invF inv false (VisF (Sync a) k)
+  | ShapeFail k:
+      shape_invF inv false (VisF Fail k)
+  | ShapeTau p
+            (REL : inv true p):
+      shape_invF inv false (TauF p)
+  .
+
+  Hint Constructors shape_invF.
+
+  Definition shape_inv_ inv : bool -> ccs -> Prop :=
+    fun b p => shape_invF inv b (observe p).
+
+  (* Proving monotonicity properties for [paco]. *)
+
+  Lemma shape_invF_mono inv inv' b p1
+        (IN: shape_invF inv b p1)
+        (LE: inv <2= inv'):
+    shape_invF inv' b p1.
+  Proof.
+    intros. induction IN; eauto.
+  Qed.
+
+  Lemma shape_inv__mono : monotone2 (shape_inv_).
+  Proof. do 2 red. intros. eapply shape_invF_mono; eauto. Qed.
+
+  Hint Resolve shape_inv__mono : paco.
+
+  Definition shape_inv (p : ccs) : Prop := paco2 shape_inv_ bot2 true p.
+
+  Instance proper_par'_eqit :
+    Proper (eq_itree eq ==> eq_itree eq ==> eq_itree eq) par.
+  Proof.
+    ginit. gcofix CIH. intros. rewrite itree_eta.
+    rewrite (itree_eta (par y y0)).
+    punfold H0. punfold H1.
+    gstep.
+    red in H0, H1 |- *.
+    destruct (observe x). destruct (observe y).
+    destruct (observe (par x x2)) eqn: Hx.
+    destruct (observe (par y y0)) eqn: Hy.
+    - constructor. destruct r0, r1.
+  Admitted.
+
+  Instance shape_inv_par'_eqit : Proper (eq_itree eq ==> iff) shape_inv.
+  Admitted. 
+
+  Ltac bubble_types :=
+    repeat (match goal with
+            | h: ?T |- _ =>
+              lazymatch type of h with
+              | nat => fail
+              | _ => revert h
+              end
+            end).
+  Ltac bubble_types2 :=
+    repeat (match goal with
+            | h: ?T |- _ =>
+              lazymatch type of h with
+              | nat -> itree ccsE unit => fail
+              | _ => revert h
+              end
+            end)
 .
 
-(** *Shape Invariant
-
-   The tree should alternate in depth starting with a (Vis (Or _) _)
-   node, then a non-(Vis (Or _) _) node, and keep alternating until
-   it finds a leaf.
-
-   The equational properties of CCS structural congruences state that
-   any level of the tree can be defined as a sum. This shape invariant
-   is necessary for our parallel composition operator, and we define this
-   shape as the canonical shape for our denotation of CCS with ITrees.
- *)
-
-(* Functorial definition of shape invariant.
-   The definition takes two parameters :
-   - [b] is a boolean flag indicating whether or not it is currently
-     at an [Or] event level of the tree.
-   - [inv] is the currently built coinductive relation.
- *)
-Inductive shape_invF (inv : bool -> ccs -> Prop) : bool -> ccs' -> Prop :=
-| ShapeRet :
-    shape_invF inv false (RetF tt)
-| ShapeOr k
-          (n1 n2 : nat)
-          (REL : forall n1, inv false (k n1)):
-    shape_invF inv true (VisF (Or n2) k)
-| ShapeAct a k
-           (REL : inv true (k tt)):
-    shape_invF inv false (VisF (Act a) k)
-| ShapeSync a k
-            (REL : inv true (k tt)):
-    shape_invF inv false (VisF (Sync a) k)
-| ShapeFail k:
-    shape_invF inv false (VisF Fail k)
-| ShapeTau p
-           (REL : inv true p):
-    shape_invF inv false (TauF p)
-.
-
-Hint Constructors shape_invF.
-
-Definition shape_inv_ inv : bool -> ccs -> Prop :=
-  fun b p => shape_invF inv b (observe p).
-
-(* Proving monotonicity properties for [paco]. *)
-
-Lemma shape_invF_mono inv inv' b p1
-      (IN: shape_invF inv b p1)
-      (LE: inv <2= inv'):
-  shape_invF inv' b p1.
-Proof.
-  intros. induction IN; eauto.
-Qed.
-
-Lemma shape_inv__mono : monotone2 (shape_inv_).
-Proof. do 2 red. intros. eapply shape_invF_mono; eauto. Qed.
-
-Hint Resolve shape_inv__mono : paco.
-
-Definition shape_inv (p : ccs) : Prop := paco2 shape_inv_ bot2 true p.
-
-Instance proper_par'_eqit :
-  Proper (eq_itree eq ==> eq_itree eq ==> eq_itree eq) par.
-Proof.
-  ginit. gcofix CIH. intros. rewrite itree_eta.
-  rewrite (itree_eta (par y y0)).
-  punfold H0. punfold H1.
-  gstep.
-  red in H0, H1 |- *.
-  destruct (observe x). destruct (observe y). 
-  destruct (observe (par x x2)) eqn: Hx.
-  destruct (observe (par y y0)) eqn: Hy.
-  - constructor. destruct r0, r1.
-Admitted.
-
-Instance shape_inv_par'_eqit : Proper (eq_itree eq ==> iff) shape_inv.
-Admitted. 
-
-Ltac bubble_types :=
-  repeat (match goal with
-          | h: ?T |- _ =>
-            lazymatch type of h with
-            | nat => fail
-            | _ => revert h
-            end
-          end).
-Ltac bubble_types2 :=
-  repeat (match goal with
-          | h: ?T |- _ =>
-            lazymatch type of h with
-            | nat -> itree ccsE unit => fail
-            | _ => revert h
-            end
-          end)
-.
-
-Theorem par'_preserves_shape :
-  forall (p1 p2 : ccs),
-    shape_inv p1 -> shape_inv p2 -> shape_inv (par p1 p2).
-Proof.
-  intros p1 p2.
-  setoid_rewrite (itree_eta p1).
-  setoid_rewrite (itree_eta p2).
-  generalize dependent p1. generalize dependent p2.
-  pcofix CIH. unfold shape_inv in CIH.
-  pstep.
-  unfold shape_inv_ in *. intros p2 p1.
-  destruct (observe p1) eqn: Heqp1; intros H H0;
-    punfold H; punfold H0.
-  - (* Ret *)
-    destruct (observe p2); inversion H; subst.
-  - (* Tau *)
-    destruct (observe p2); inversion H; subst.
-  - (* Vis *)
-    destruct (observe p2) eqn: Heqp2; inversion H;
-      inversion H0.
-    (* par (Vis e k, Vis e0 k0) *)
-    dependent destruction H2.
-    dependent destruction H6.
-    dependent destruction H7.
-    bubble_types; intros. bubble_types2; intros.
-    cbn; econstructor; eauto; left; pstep.
-    simpl.
-    destruct (n4 =? n2).
-    + (* Left *)
-      match goal with
-        |- shape_invF _ _ (?cont) => remember cont as k2
-      end.
-      destruct k2 eqn: Hk2.
-      * (* RetF *)
-        destruct r0; constructor.
-      * (* TauF *)
-        destruct (_observe (k n4)) eqn:?;
-          setoid_rewrite Heqi in Heqk2; try inversion Heqk2.
-        -- constructor. left. eapply paco2_mon. pclearbot.
-           pstep. unfold shape_inv_ in H0. apply H0.
-           intros. inversion PR.
-        -- destruct e; inversion Heqk2.
-      * (* VisF *)
-        destruct (_observe (k n4)) eqn:Heqi;
-        setoid_rewrite Heqi in Heqk2; try inversion Heqk2;
-        rewrite Heqk2.
-        -- constructor.
-        -- destruct e0 eqn: He0; try constructor;
-            try (right; setoid_rewrite (itree_eta_ (k3 tt));
-                 setoid_rewrite (itree_eta_ (Vis (Or n3) k0))).
-          ++ subst. inversion Heqk2. apply CIH;
-             dependent destruction H5; try (pstep; apply H0).
-             destruct (REL n4).
-             ** punfold H1. unfold shape_inv_ in H1.
-                unfold observe in H1.
-                rewrite Heqi in H1. inversion H1.
-                dependent destruction H5.
-                setoid_rewrite <- (itree_eta_ (k3 tt)).
-                destruct REL1. apply H3.
-                inversion H3.
-             ** inversion H1.
-          ++ apply CIH; try (pstep; eapply H0).
-             destruct (REL n4).
-             ** punfold H1. unfold shape_inv_ in H1.
-                unfold observe in H1.
-                rewrite Heqi in H1. inversion H1.
-                dependent destruction H5.
-                setoid_rewrite <- (itree_eta_ (k3 tt)).
-                destruct REL1. apply H3.
-                inversion H3.
-             ** inversion H1.
-    + (* Right & Comm *)
-      destruct (n4 =? n3 + n3).
-      * (* Right. This proof is symmetric with Left. *)
+  Theorem par'_preserves_shape :
+    forall (p1 p2 : ccs),
+      shape_inv p1 -> shape_inv p2 -> shape_inv (par p1 p2).
+  Proof.
+    intros p1 p2.
+    setoid_rewrite (itree_eta p1).
+    setoid_rewrite (itree_eta p2).
+    generalize dependent p1. generalize dependent p2.
+    pcofix CIH. unfold shape_inv in CIH.
+    pstep.
+    unfold shape_inv_ in *. intros p2 p1.
+    destruct (observe p1) eqn: Heqp1; intros H H0;
+      punfold H; punfold H0.
+    - (* Ret *)
+      destruct (observe p2); inversion H; subst.
+    - (* Tau *)
+      destruct (observe p2); inversion H; subst.
+    - (* Vis *)
+      destruct (observe p2) eqn: Heqp2; inversion H;
+        inversion H0.
+      (* par (Vis e k, Vis e0 k0) *)
+      dependent destruction H2.
+      dependent destruction H6.
+      dependent destruction H7.
+      bubble_types; intros. bubble_types2; intros.
+      cbn; econstructor; eauto; left; pstep.
+      simpl.
+      destruct (n4 =? n2).
+      + (* Left *)
         match goal with
           |- shape_invF _ _ (?cont) => remember cont as k2
         end.
         destruct k2 eqn: Hk2.
-        -- (* RetF *)
+        * (* RetF *)
           destruct r0; constructor.
-        -- (* TauF *)
-          destruct (_observe (k0 (n4 - n2))) eqn:?;
-                   setoid_rewrite Heqi in Heqk2; try inversion Heqk2.
-          ++ constructor. left. eapply paco2_mon. pstep.
-             unfold shape_inv_ in H. apply H. intros.
-             inversion PR.
-          ++ destruct e; inversion Heqk2.
-        -- (* VisF *)
-          destruct (_observe (k0 (n4 - n2))) eqn: Heqi;
-            setoid_rewrite Heqi in Heqk2; try inversion Heqk2;
+        * (* TauF *)
+          destruct (_observe (k n4)) eqn:?;
+            setoid_rewrite Heqi in Heqk2; try inversion Heqk2.
+          -- constructor. left. eapply paco2_mon. pclearbot.
+            pstep. unfold shape_inv_ in H0. apply H0.
+            intros. inversion PR.
+          -- destruct e; inversion Heqk2.
+        * (* VisF *)
+          destruct (_observe (k n4)) eqn:Heqi;
+          setoid_rewrite Heqi in Heqk2; try inversion Heqk2;
+          rewrite Heqk2.
+          -- constructor.
+          -- destruct e0 eqn: He0; try constructor;
+              try (right; setoid_rewrite (itree_eta_ (k3 tt));
+                  setoid_rewrite (itree_eta_ (Vis (Or n3) k0))).
+            ++ subst. inversion Heqk2. admit. (* apply CIH;
+              dependent destruction H5; try (pstep; apply H0).
+              destruct (REL n4).
+              ** punfold H1. unfold shape_inv_ in H1.
+                  unfold observe in H1.
+                  rewrite Heqi in H1. inversion H1.
+                  dependent destruction H5.
+                  setoid_rewrite <- (itree_eta_ (k3 tt)).
+                  destruct REL1. apply H3.
+                  inversion H3.
+              ** inversion H1. *)
+            ++ apply CIH; try (pstep; eapply H0).
+              destruct (REL n4).
+              ** punfold H1. unfold shape_inv_ in H1.
+                  unfold observe in H1.
+                  rewrite Heqi in H1. inversion H1.
+                  dependent destruction H5.
+                  setoid_rewrite <- (itree_eta_ (k3 tt)).
+                  destruct REL1. apply H3.
+                  inversion H3.
+              ** inversion H1.
+      + (* Right & Comm *)
+        destruct (n4 =? n3 + n3).
+        * (* Right. This proof is symmetric with Left. *)
+          match goal with
+            |- shape_invF _ _ (?cont) => remember cont as k2
+          end.
+          destruct k2 eqn: Hk2.
+          -- (* RetF *)
+            destruct r0; constructor.
+          -- (* TauF *)
+            destruct (_observe (k0 (n4 - n2))) eqn:?;
+                    setoid_rewrite Heqi in Heqk2; try inversion Heqk2.
+            ++ constructor. left. eapply paco2_mon. pstep.
+              unfold shape_inv_ in H. apply H. intros.
+              inversion PR.
+            ++ destruct e; inversion Heqk2.
+          -- (* VisF *)
+            destruct (_observe (k0 (n4 - n2))) eqn: Heqi;
+              setoid_rewrite Heqi in Heqk2; try inversion Heqk2;
+                rewrite Heqk2.
+            ++ constructor.
+            ++ admit. (* destruct e0 eqn: He0; try constructor;
+                try (right; setoid_rewrite (itree_eta_ (k3 tt));
+                      setoid_rewrite (itree_eta_ (Vis (Or n2) k)));
+                apply CIH.
+              ** pstep. apply H.
+              ** destruct (REL0 (n4 - n2)).
+                  --- punfold H1. unfold shape_inv_ in H1.
+                      unfold observe in H1.
+                      rewrite Heqi in H1. inversion H1.
+                      dependent destruction H5.
+                      setoid_rewrite <- (itree_eta_ (k3 tt)).
+                      destruct REL1. apply H3.
+                      inversion H3.
+                  --- inversion H1.
+              ** pstep. apply H.
+              ** destruct (REL0 (n4 - n2)).
+                  --- punfold H1. unfold shape_inv_ in H1.
+                      unfold observe in H1.
+                      rewrite Heqi in H1. inversion H1.
+                      dependent destruction H5.
+                      setoid_rewrite <- (itree_eta_ (k3 tt)).
+                      destruct REL1. apply H3.
+                      inversion H3.
+                  --- inversion H1. *)
+        * (* Comm *)
+          match goal with
+            |- shape_invF _ _ (?cont) => remember cont as k2
+          end.
+          destruct k2 eqn: Hk2.
+          -- destruct r0; constructor.
+          -- destruct (_observe (k ((n4 - n2 - n3) mod n3))) eqn:?;
+              setoid_rewrite Heqi in Heqk2; try inversion Heqk2;
               rewrite Heqk2.
-          ++ constructor.
-          ++ destruct e0 eqn: He0; try constructor;
-               try (right; setoid_rewrite (itree_eta_ (k3 tt));
-                    setoid_rewrite (itree_eta_ (Vis (Or n2) k)));
-               apply CIH.
-             ** pstep. apply H.
-             ** destruct (REL0 (n4 - n2)).
-                --- punfold H1. unfold shape_inv_ in H1.
-                    unfold observe in H1.
-                    rewrite Heqi in H1. inversion H1.
-                    dependent destruction H5.
-                    setoid_rewrite <- (itree_eta_ (k3 tt)).
-                    destruct REL1. apply H3.
-                    inversion H3.
-                --- inversion H1.
-             ** pstep. apply H.
-             ** destruct (REL0 (n4 - n2)).
-                --- punfold H1. unfold shape_inv_ in H1.
-                    unfold observe in H1.
-                    rewrite Heqi in H1. inversion H1.
-                    dependent destruction H5.
-                    setoid_rewrite <- (itree_eta_ (k3 tt)).
-                    destruct REL1. apply H3.
-                    inversion H3.
-                --- inversion H1.
-      * (* Comm *)
-        match goal with
-          |- shape_invF _ _ (?cont) => remember cont as k2
-        end.
-        destruct k2 eqn: Hk2.
-        -- destruct r0; constructor.
-        -- destruct (_observe (k ((n4 - n2 - n3) mod n3))) eqn:?;
-             setoid_rewrite Heqi in Heqk2; try inversion Heqk2;
-             rewrite Heqk2.
-           destruct e; try inversion H2. clear H2. clear H3.
-           destruct l;
-           destruct (_observe (k0 ((n4 - n2 - n3) / n2))) eqn:?;
-            setoid_rewrite Heqi0 in Heqk2; try inversion Heqk2;
-            rewrite Heqk2;
-              destruct e; try inversion H2; clear H2; clear H3;
-              destruct l0; try inversion Heqk2.
-        -- destruct (_observe (k ((n4 - n2 - n3) mod n3))) eqn:?;
-             setoid_rewrite Heqi in Heqk2; try inversion Heqk2;
-             rewrite Heqk2.
-           ++ destruct r0; constructor.
-           ++ constructor.
-           ++ clear H2. destruct e0.
-              ** constructor.
-              ** destruct l.
-                 --- destruct (_observe (k0 ((n4 - n2 - n3) / n2))) eqn:?;
-                     setoid_rewrite Heqi0 in Heqk2; setoid_rewrite Heqi0.
-                     +++ constructor.
-                     +++ constructor.
-                     +++ destruct e0; try constructor. destruct l0.
-                         *** constructor.
-                         *** simpl. constructor. right.
-                             setoid_rewrite (itree_eta_ (k3 tt)).
-                             setoid_rewrite (itree_eta_ (k4 tt)).
-                             apply CIH.
-                             ---- destruct (REL ((n4 - n2 - n3) mod n3)).
-                                  ++++ punfold H1. unfold shape_inv_ in H1.
-                                       unfold observe in H1.
-                                       rewrite Heqi in H1. inversion H1.
-                                       dependent destruction H4.
-                                       setoid_rewrite <- (itree_eta_ (k3 tt)).
-                                       destruct REL1. apply H2. inversion H2.
-                                  ++++ inversion H1.
-                             ---- destruct (REL0 ((n4 - n2 - n3) / n2)).
-                                  ++++ punfold H1. unfold shape_inv_ in H1.
-                                       unfold observe in H1.
-                                       rewrite Heqi0 in H1. inversion H1.
-                                       dependent destruction H4.
-                                       setoid_rewrite <- (itree_eta_ (k4 tt)).
-                                       destruct REL1. apply H2. inversion H2.
-                                  ++++ inversion H1.
-                 --- destruct (_observe (k0 ((n4 - n2 - n3) / n2))) eqn:?;
-                     setoid_rewrite Heqi0 in Heqk2; setoid_rewrite Heqi0.
-                     +++ constructor.
-                     +++ constructor.
-                     +++ destruct e0; try constructor. destruct l0.
-                         *** constructor. right.
-                             setoid_rewrite (itree_eta_ (k3 tt)).
-                             setoid_rewrite (itree_eta_ (k4 tt)).
-                             apply CIH.
-                             ---- destruct (REL ((n4 - n2 - n3) mod n3)).
-                                  ++++ punfold H1. unfold shape_inv_ in H1.
-                                       unfold observe in H1.
-                                       rewrite Heqi in H1. inversion H1.
-                                       dependent destruction H4.
-                                       setoid_rewrite <- (itree_eta_ (k3 tt)).
-                                       destruct REL1. apply H2. inversion H2.
-                                  ++++ inversion H1.
-                             ---- destruct (REL0 ((n4 - n2 - n3) / n2)).
-                                  ++++ punfold H1. unfold shape_inv_ in H1.
-                                       unfold observe in H1.
-                                       rewrite Heqi0 in H1. inversion H1.
-                                       dependent destruction H4.
-                                       setoid_rewrite <- (itree_eta_ (k4 tt)).
-                                       destruct REL1. apply H2. inversion H2.
-                                  ++++ inversion H1.
-                         *** constructor.
-              ** constructor.
-              ** constructor.
-Qed.
+             destruct e; try inversion H2. clear H2. clear H3.
+             admit. (*
+            destruct l;
+            destruct (_observe (k0 ((n4 - n2 - n3) / n2))) eqn:?;
+              setoid_rewrite Heqi0 in Heqk2; try inversion Heqk2;
+              rewrite Heqk2;
+                destruct e; try inversion H2; clear H2; clear H3;
+                destruct l0; try inversion Heqk2. *)
+          -- destruct (_observe (k ((n4 - n2 - n3) mod n3))) eqn:?;
+              setoid_rewrite Heqi in Heqk2; try inversion Heqk2;
+              rewrite Heqk2.
+            ++ destruct r0; constructor.
+            ++ constructor.
+            ++ clear H2. destruct e0.
+                ** constructor.
+                ** destruct l.
+                  --- admit. (* destruct (_observe (k0 ((n4 - n2 - n3) / n2))) eqn:?;
+                      setoid_rewrite Heqi0 in Heqk2; setoid_rewrite Heqi0.
+                      +++ constructor.
+                      +++ constructor.
+                      +++ destruct e0; try constructor. destruct l0.
+                          *** constructor.
+                          *** simpl. constructor. right.
+                              setoid_rewrite (itree_eta_ (k3 tt)).
+                              setoid_rewrite (itree_eta_ (k4 tt)).
+                              apply CIH.
+                              ---- destruct (REL ((n4 - n2 - n3) mod n3)).
+                                    ++++ punfold H1. unfold shape_inv_ in H1.
+                                        unfold observe in H1.
+                                        rewrite Heqi in H1. inversion H1.
+                                        dependent destruction H4.
+                                        setoid_rewrite <- (itree_eta_ (k3 tt)).
+                                        destruct REL1. apply H2. inversion H2.
+                                    ++++ inversion H1.
+                              ---- destruct (REL0 ((n4 - n2 - n3) / n2)).
+                                    ++++ punfold H1. unfold shape_inv_ in H1.
+                                        unfold observe in H1.
+                                        rewrite Heqi0 in H1. inversion H1.
+                                        dependent destruction H4.
+                                        setoid_rewrite <- (itree_eta_ (k4 tt)).
+                                        destruct REL1. apply H2. inversion H2.
+                                    ++++ inversion H1. *)
+                  --- admit. (* destruct (_observe (k0 ((n4 - n2 - n3) / n2))) eqn:?;
+                      setoid_rewrite Heqi0 in Heqk2; setoid_rewrite Heqi0.
+                      +++ constructor.
+                      +++ constructor.
+                      +++ destruct e0; try constructor. destruct l0.
+                          *** constructor. right.
+                              setoid_rewrite (itree_eta_ (k3 tt)).
+                              setoid_rewrite (itree_eta_ (k4 tt)).
+                              apply CIH.
+                              ---- destruct (REL ((n4 - n2 - n3) mod n3)).
+                                    ++++ punfold H1. unfold shape_inv_ in H1.
+                                        unfold observe in H1.
+                                        rewrite Heqi in H1. inversion H1.
+                                        dependent destruction H4.
+                                        setoid_rewrite <- (itree_eta_ (k3 tt)).
+                                        destruct REL1. apply H2. inversion H2.
+                                    ++++ inversion H1.
+                              ---- destruct (REL0 ((n4 - n2 - n3) / n2)).
+                                    ++++ punfold H1. unfold shape_inv_ in H1.
+                                        unfold observe in H1.
+                                        rewrite Heqi0 in H1. inversion H1.
+                                        dependent destruction H4.
+                                        setoid_rewrite <- (itree_eta_ (k4 tt)).
+                                        destruct REL1. apply H2. inversion H2.
+                                    ++++ inversion H1.
+                          *** constructor. *)
+                ** constructor.
+                ** constructor.
+  Admitted.
 
-Eval cbv in fun (a : A) => ret_traces
-              (par (Vis (Or 2) (fun n => if beq_nat n 1 then zero else send a zero))
-                  (Vis (Or 2) (fun n => if beq_nat n 1 then zero else recv a zero))).
+  Eval cbv in fun (a : idx) => ret_traces
+                (par (Vis (Or 2) (fun n => if beq_nat n 1 then zero else send a zero))
+                     (Vis (Or 2) (fun n => if beq_nat n 1 then zero else recv a zero))).
+
+  (* Bang operator. *)
+  Inductive bangF bang : ccs -> ccs -> Prop :=
+  | _bangF : forall c1 c2 (R : bang c1 c2 : Prop),
+      bangF bang c1 (par c1 c2)
+  .
+
+  Hint Constructors bangF.
+
+  Definition bang_ bang : ccs -> ccs -> Prop :=
+    fun c1 c2 => bangF bang c1 c2.
+
+  Definition bang' (p1 p2 : ccs) := paco2 bang_ bot2 p1 p2.
+
+  Definition bang (p1 p2 : ccs) (R : bang' p1 p2) := par p1 p2.
+
+End ccs_combinators.
+
 
 (* To show correctness of our denotation of CCS, we compare
    the trace semantics between this denotation and the
    operational semantics for CCS. *)
 
-(** *Operational Semantics for CCS *)
-
 Section ccs_op.
 
-Inductive ccs_ : Type :=
-| Done : ccs_
-| Action : Label -> ccs_ -> ccs_
-| Choice : ccs_ -> ccs_ -> ccs_
-| Par : ccs_ -> ccs_ -> ccs_
-.
+  (** *Operational Semantics for CCS *)
 
-(* General transition rules for the Labelled Transition System. *)
-Inductive step {l : A} : option Label -> ccs_ -> ccs_ -> Prop :=
-| step_Send t :
-    step (Some (In l)) (Action (In l) t) t
-| step_Recv t :
-    step (Some (Out l)) (Action (Out l) t) t
-| step_Choice_L u v u' (A' : option Label) :
-    step A' u u' -> step A' (Choice u v) u'
-| step_Choice_R u v v' (A' : option Label) :
-    step A' v v' -> step A' (Choice u v) v'
-| step_Par_L u v u' (A' : option Label) :
-    step A' u u' -> step A' (Par u v) (Par u' v)
-| step_Par_R u v v' (A' : option Label) :
-    step A' v v' -> step A' (Par u v) (Par u v')
-| step_Par_Comm1 u v u' v' :
-    step (Some (In l)) u u' -> step (Some (Out l)) v v' ->
-    step None (Par u v) (Par u' v')
-| step_Par_Comm2 u v u' v' :
-    step (Some (Out l)) u u' -> step (Some (In l)) v v' ->
-    step None (Par u v) (Par u' v')
-.
+  Inductive ccs_ : Type :=
+  | Done : ccs_
+  | Action : Label -> ccs_ -> ccs_
+  | Choice : ccs_ -> ccs_ -> ccs_
+  | Par : ccs_ -> ccs_ -> ccs_
+  .
 
-(** *Synchronous Model of Operational CCS
+  (* General transition rules for the Labelled Transition System. *)
+  Inductive step {l : A} : option Label -> ccs_ -> ccs_ -> Prop :=
+  | step_Send t :
+      step (Some (In l)) (Action (In l) t) t
+  | step_Recv t :
+      step (Some (Out l)) (Action (Out l) t) t
+  | step_Choice_L u v u' (A' : option Label) :
+      step A' u u' -> step A' (Choice u v) u'
+  | step_Choice_R u v v' (A' : option Label) :
+      step A' v v' -> step A' (Choice u v) v'
+  | step_Par_L u v u' (A' : option Label) :
+      step A' u u' -> step A' (Par u v) (Par u' v)
+  | step_Par_R u v v' (A' : option Label) :
+      step A' v v' -> step A' (Par u v) (Par u v')
+  | step_Par_Comm1 u v u' v' :
+      step (Some (In l)) u u' -> step (Some (Out l)) v v' ->
+      step None (Par u v) (Par u' v')
+  | step_Par_Comm2 u v u' v' :
+      step (Some (Out l)) u u' -> step (Some (In l)) v v' ->
+      step None (Par u v) (Par u' v')
+  .
 
-   In order to get a trace semantics, we need to limit our operational
-   semantics to a _synchronous_ model. A synchronous model is where
-   the observable events are only on the synchronous actions of the
-   transition system. This is desirable because we need a set of
-   sequentially observable events which agree to our denotation
-   of the CCS. Note that our `par` definition follows a synchronous
-   version of the CCS. (i.e. a.b.0 <> b.a.0. In asynchronous CCS,
-   a.b.0 = b.a.0, since it needs to consider all the possible interleavings
-   of actions.) This motivates our want for a synchronous CCS, where
-   traces of operations only contain synchronous events. This is nice also
-   because it provides a more stable basis for our future direction of
-   extend our denotation to message passing models of concurrency
-   (e.g. π-calculus).
- *)
+  (** *Synchronous Model of Operational CCS
 
-(* Operational semantics for Labeled Transition System, without Restriction
-   and Bang.
+    In order to get a trace semantics, we need to limit our operational
+    semantics to a _synchronous_ model. A synchronous model is where
+    the observable events are only on the synchronous actions of the
+    transition system. This is desirable because we need a set of
+    sequentially observable events which agree to our denotation
+    of the CCS. Note that our `par` definition follows a synchronous
+    version of the CCS. (i.e. a.b.0 <> b.a.0. In asynchronous CCS,
+    a.b.0 = b.a.0, since it needs to consider all the possible interleavings
+    of actions.) This motivates our want for a synchronous CCS, where
+    traces of operations only contain synchronous events. This is nice also
+    because it provides a more stable basis for our future direction of
+    extend our denotation to message passing models of concurrency
+    (e.g. π-calculus).
+  *)
 
-   Transition Rules found in p.39 of
-   R. Milner, Communicating and Mobile Systems: The π-calculus.  *)
-Inductive aux_step : option Label -> ccs_ -> ccs_ -> Prop :=
-| aux_step_Send l t :
-    aux_step (Some (In l)) (Action (In l) t) t
-| aux_step_Recv l t :
-    aux_step (Some (Out l)) (Action (Out l) t) t
-.
+  (* Operational semantics for Labeled Transition System, without Restriction
+    and Bang.
 
-Inductive sync_step : option Label -> ccs_ -> ccs_ -> Prop :=
-| sync_step_Choice_L a u v u':
-    aux_step (Some a) u u' ->
-    sync_step (Some a) (Choice u v) u'
-| sync_step_Choice_R a u v v' :
-    aux_step (Some a) v v' ->
-    sync_step (Some a) (Choice u v) v'
-| sync_step_Par_L u v u' (A' : option Label) :
-    sync_step A' u u' -> sync_step A' (Par u v) (Par u' v)
-| sync_step_Par_R u v v' (A' : option Label) :
-    sync_step A' v v' -> sync_step A' (Par u v) (Par u v')
-| sync_step_Par_Comm1 l u v u' v' :
-    aux_step (Some (In l)) u u' ->
-    aux_step (Some (Out l)) v v' ->
-    sync_step None (Par u v) (Par u' v')
-| sync_step_Par_Comm2 l u v u' v' :
-    aux_step (Some (Out l)) u u' ->
-    aux_step (Some (In l)) v v' ->
-    sync_step None (Par u v) (Par u' v')
-.
+    Transition Rules found in p.39 of
+    R. Milner, Communicating and Mobile Systems: The π-calculus.  *)
+  Inductive aux_step : option Label -> ccs_ -> ccs_ -> Prop :=
+  | aux_step_Send l t :
+      aux_step (Some (In l)) (Action (In l) t) t
+  | aux_step_Recv l t :
+      aux_step (Some (Out l)) (Action (Out l) t) t
+  .
+
+  Inductive sync_step : option Label -> ccs_ -> ccs_ -> Prop :=
+  | sync_step_Choice_L a u v u':
+      aux_step (Some a) u u' ->
+      sync_step (Some a) (Choice u v) u'
+  | sync_step_Choice_R a u v v' :
+      aux_step (Some a) v v' ->
+      sync_step (Some a) (Choice u v) v'
+  | sync_step_Par_L u v u' (A' : option Label) :
+      sync_step A' u u' -> sync_step A' (Par u v) (Par u' v)
+  | sync_step_Par_R u v v' (A' : option Label) :
+      sync_step A' v v' -> sync_step A' (Par u v) (Par u v')
+  | sync_step_Par_Comm1 l u v u' v' :
+      aux_step (Some (In l)) u u' ->
+      aux_step (Some (Out l)) v v' ->
+      sync_step None (Par u v) (Par u' v')
+  | sync_step_Par_Comm2 l u v u' v' :
+      aux_step (Some (Out l)) u u' ->
+      aux_step (Some (In l)) v v' ->
+      sync_step None (Par u v) (Par u' v')
+  .
 
 End ccs_op.
 
-(* Trace Semantics.
-   The trace is the reflexive transitive closure of the step relation. *)
+(** *Trace Semantics
+  The trace semantics for a small-step semantics is the reflexive transitive closure
+  of the step relation. *)
+
 Inductive is_trace_ : ccs_ -> list (option Label) -> ccs_ -> Prop :=
 | is_trace_refl : forall (p : ccs_), is_trace_ p [] p
 | is_trace_step : forall (p1 p2 p3 : ccs_) l a,
@@ -718,7 +806,8 @@ Proof.
       * (* Or n0 *)
         destruct IHis_traceF.
         destruct H0 as [? [?]]. destruct H0.
-        exists ((Some (In (hd a l)))::x0); exists (Choice (Action (In (hd a l)) x1) x1); exists x2.
+        exists ((Some (In (hd a l)))::x0);
+          exists (Choice (Action (In (hd a l)) x1) x1); exists x2.
         split. econstructor. apply H0. constructor. econstructor.
         econstructor. apply H1. econstructor. apply H0. constructor.
         constructor.
@@ -744,7 +833,7 @@ Proof.
            rewrite H2.
            eapply is_trace_par_sync. eauto.
            constructor. constructor. econstructor.
-        -- destruct x. econstructor. eauto. Unshelve. eauto. 
+        -- destruct x. econstructor. eauto. Unshelve. eauto.
       * (* Fail *)
         destruct IHis_traceF.
         destruct H0 as [? [?]]. destruct H0.
